old/matroid_intersection.lean
@@ -126,7 +126,7 @@ begin
     rw [←size_largest_common_ind_eq_nu, ←hIc, hk], 
     linarith 
     [
-      add_nonmem_size heIc,
+      size_insert_nonmem heIc,
       size_common_ind_le_nu 
       ⟨
         indep_of_project_indep hIc'.1 (nonloop_iff_indep.mp h_e_nl.1), 
@@ -143,7 +143,7 @@ begin
       (loopify_makes_loops N₂ e), 
     rw ←union_distrib_union_left at h_add_e, 
     have := size_monotone h_add_e, 
-    rw [add_compl_single_size he, ←hN₁d, ←hN₂d] at this, 
+    rw [size_insert_mem_compl he, ←hN₁d, ←hN₂d] at this, 
     rw [compl_size] at ⊢ hsize, linarith,  
   },
 
@@ -154,7 +154,7 @@ begin
       (project_makes_loops N₂ e), 
     rw ←union_distrib_union_left at h_add_e, 
     have := size_monotone h_add_e, 
-    rw [add_compl_single_size he, ←hN₁c, ←hN₂c] at this, 
+    rw [size_insert_mem_compl he, ←hN₁c, ←hN₂c] at this, 
     rw [compl_size] at ⊢ hsize, linarith,  
   },  
   
