src/prelim/induction.lean
@@ -98,7 +98,7 @@ begin
   refine nonneg_int_strong_induction_param P size (size_nonneg) (λ X hX, _) (λ X hX hX', _ ), 
   { convert h0, apply size_zero_empty hX}, 
   rcases size_pos_iff_has_mem.mp hX with ⟨e,he⟩, 
-  exact h X ⟨e,he⟩ (hX' (X \ {e}) (by linarith [remove_single_size he])), 
+  exact h X ⟨e,he⟩ (hX' (X \ {e}) (by linarith [size_remove_mem he])), 
 end
 
 lemma induction_set_size_add (P : set A → Prop): 
@@ -109,7 +109,7 @@ begin
   { convert h0, apply size_zero_empty hX}, 
   rcases size_pos_iff_has_mem.mp hX with ⟨e,he⟩, 
   convert h (X \ {e}) e _ (hX' _ _);
-  simp [insert_eq_of_mem he, int.zero_lt_one,remove_single_size he], 
+  simp [insert_eq_of_mem he, int.zero_lt_one,size_remove_mem he], 
 end
 
 end numbers 
